TM/Prelim.v
@@ -403,13 +403,13 @@ Tactic Notation "spec_assert" hyp(H) "by" tactic(T) :=
     assert A as H' by T; specialize (H H'); clear H'
   end.
 
+
 Tactic Notation "spec_assert" hyp(H) "as" simple_intropattern(p) "by" tactic(T) :=
   let H' := fresh in
   match type of H with
   | ?A -> _ =>
-    assert A as H' by T; [ | specialize (H H') as p; clear H']
+    assert A as H' by T; specialize (H H') as p; clear H'
   end.
-
 
 
 (* Dupfree vector *)
